Add ugly proof of countability for formulas

Fine/PropositionalLanguage.lean
@@ -1,11 +1,12 @@
 import Mathlib.Init.Set
+import Mathlib.Logic.Denumerable
 
 inductive Form : Type
   | atom : Nat → Form
-  | impl : Form → Form → Form
+  | neg  : Form → Form
   | and  : Form → Form → Form
   | or   : Form → Form → Form
-  | neg  : Form → Form
+  | impl : Form → Form → Form
   deriving DecidableEq
 
 prefix:max "#" => Form.atom
@@ -14,6 +15,84 @@ infixr:512 "&" => Form.and
 infixr:512 "¦" => Form.or
 prefix:max "~" => Form.neg
 
+abbrev tupleEquiv := Nat⊕ Nat⊕ (Nat × Nat)⊕ (Nat × Nat)⊕ (Nat×Nat)
+
+def toSumEncoding : Form → Nat⊕ Nat⊕ (Nat × Nat)⊕ (Nat × Nat)⊕ (Nat×Nat)
+    | #n => Sum.inl n
+    | ~f => Sum.inr $ Sum.inl (Encodable.encode $ toSumEncoding f)
+    | f & g => Sum.inr $ Sum.inr $ Sum.inl ⟨Encodable.encode $ toSumEncoding f, Encodable.encode $ toSumEncoding g⟩
+    | f ¦ g => Sum.inr $ Sum.inr $ Sum.inr $ Sum.inl ⟨Encodable.encode $ toSumEncoding f, Encodable.encode $ toSumEncoding g⟩
+    | Form.impl f g => Sum.inr $ Sum.inr $ Sum.inr $ Sum.inr ⟨Encodable.encode $ toSumEncoding f, Encodable.encode $ toSumEncoding g⟩
+
+theorem sum_encoding_injection : Function.Injective toSumEncoding := by
+  unfold Function.Injective
+  intros P
+  induction P
+  case atom n =>
+    intros Q h₁
+    cases Q
+    · unfold toSumEncoding at h₁
+      injection h₁ with h₁
+      rw [h₁]
+    repeat (unfold toSumEncoding at h₁; injection h₁)
+  case neg Q ih =>
+    intros R h
+    cases R
+    case neg S =>
+      unfold toSumEncoding at h
+      repeat (injection h with h)
+      have l := ih (Encodable.encode_injective h)
+      simp [l]
+    repeat
+      unfold toSumEncoding at h
+      repeat (injection h with h)
+      injection h
+  case and =>
+    rename_i R S ih₁ ih₂
+    intros T h₁
+    cases T
+    case and U V =>
+      unfold toSumEncoding at h₁
+      repeat (injection h₁ with h₁)
+      rename_i h₂
+      have l₁ := ih₁ (Encodable.encode_injective h₁)
+      have l₂ := ih₂ (Encodable.encode_injective h₂)
+      simp [l₁,l₂]
+    repeat
+      unfold toSumEncoding at h₁
+      repeat (injection h₁ with h₁)
+      injection h₁
+  case or =>
+    rename_i R S ih₁ ih₂
+    intros T h₁
+    cases T
+    case or U V =>
+      unfold toSumEncoding at h₁
+      repeat (injection h₁ with h₁)
+      rename_i h₂
+      have l₁ := ih₁ (Encodable.encode_injective h₁)
+      have l₂ := ih₂ (Encodable.encode_injective h₂)
+      simp [l₁,l₂]
+    repeat
+      unfold toSumEncoding at h₁
+      repeat (injection h₁ with h₁)
+      injection h₁
+  case impl => 
+    rename_i R S ih₁ ih₂
+    intros T h₁
+    cases T
+    case impl U V =>
+      unfold toSumEncoding at h₁
+      repeat (injection h₁ with h₁)
+      rename_i h₂
+      have l₁ := ih₁ (Encodable.encode_injective h₁)
+      have l₂ := ih₂ (Encodable.encode_injective h₂)
+      simp [l₁,l₂]
+    repeat
+      unfold toSumEncoding at h₁
+      repeat (injection h₁ with h₁)
+      injection h₁
+    
 instance : ToString Form where
   toString := display
   where display: Form → String
